more

Weidenbach_Book/CDCL_Two_Watched_Literals_List_Watched_Domain.thy
@@ -348,58 +348,39 @@ locale twl_array_code =
   assumes in_N1_less_than_upperN: \<open>\<forall>L \<in># N\<^sub>1. nat_of_lit L < upperN\<close>
 begin
 
-definition unit_propagation_inner_loop_body_wl_D :: "nat literal \<Rightarrow> nat \<Rightarrow>
-  nat twl_st_wl \<Rightarrow> (nat \<times> nat twl_st_wl) nres"  where
-  \<open>unit_propagation_inner_loop_body_wl_D K w S = do {
-    ASSERT(unit_prop_body_wl_inv S w K);
-    ASSERT(literals_are_N\<^sub>0 S);
-    let (M, N, U, D', NP, UP, Q, W) = S;
-    ASSERT(K \<in># all_lits_of_mm (mset `# mset (tl N) + NP));
-    ASSERT(w < length (watched_by S K));
-    ASSERT(K \<in> snd ` D\<^sub>0);
-    let C = (W K) ! w;
-    ASSERT(C > 0);
-    ASSERT(no_dup M);
-    ASSERT(C < length N);
-    ASSERT(0 < length (N!C));
-    let i = (if (N!C) ! 0 = K then 0 else 1);
-    ASSERT(i < length (N!C));
-    ASSERT(1-i < length (N!C));
-    let L = K;
-    let L' = (N!C) ! (1 - i);
-    ASSERT(L' \<in># mset (watched_l (N!C)) - {#L#});
-    ASSERT (mset (watched_l (N!C)) = {#L, L'#});
-    ASSERT(L' \<in> snd ` D\<^sub>0);
-    val_L' \<leftarrow> RETURN (valued M L');
-    if val_L' = Some True
-    then RETURN (w+1, (M, N, U, D', NP, UP, Q, W))
-    else do {
-      ASSERT(literals_are_in_N\<^sub>0 (mset (N!C)));
-      f \<leftarrow> find_unwatched M (N!C);
-      ASSERT (f = None \<longleftrightarrow> (\<forall>L\<in>#mset (unwatched_l (N!C)). - L \<in> lits_of_l M));
-      case f of
-        None \<Rightarrow>
-          if val_L' = Some False
-          then do {RETURN (w+1, (M, N, U, Some (mset (N!C)), NP, UP, {#}, W))}
-          else do {
-            ASSERT(undefined_lit M L');
-            RETURN (w+1, (Propagated L' C # M, N, U, D', NP, UP, add_mset (-L') Q, W))}
-      | Some f \<Rightarrow> do {
-           ASSERT(f < length (N!C));
-           let K' = (N!C) ! f;
-           ASSERT(K' \<in># all_lits_of_mm (mset `# mset (tl N) + NP));
-           ASSERT(K' \<in> snd ` D\<^sub>0);
-           let N' = list_update N C (swap (N!C) i f);
-           let W = W(L := delete_index_and_swap (W L) w);
-           let W = W(K':= W K' @ [C]);
-           ASSERT(K \<noteq> K');
-           RETURN (w, (M, N', U, D', NP, UP, Q, W))
-       }
-    }
-   }
-\<close>
+definition unit_prop_body_wl_D_inv where
+\<open>unit_prop_body_wl_D_inv T' i L \<longleftrightarrow>
+    unit_prop_body_wl_inv T' i L \<and> literals_are_N\<^sub>0 T' \<and> L \<in> snd ` D\<^sub>0
+  \<close>
 
-lemma mset_tl_update_swap:
+definition unit_propagation_inner_loop_body_wl_D :: "nat literal \<Rightarrow> nat \<Rightarrow> nat twl_st_wl \<Rightarrow>
+    (nat \<times> nat twl_st_wl) nres" where
+  \<open>unit_propagation_inner_loop_body_wl_D L w S = do {
+      ASSERT(unit_prop_body_wl_D_inv S w L);
+      let C = (watched_by S L) ! w;
+      let i = (if ((get_clauses_wl S)!C) ! 0 = L then 0 else 1);
+      let L' = ((get_clauses_wl S)!C) ! (1 - i);
+      let val_L' = valued (get_trail_wl S) L';
+      if val_L' = Some True
+      then RETURN (w+1, S)
+      else do {
+        f \<leftarrow> find_unwatched_l (get_trail_wl S) ((get_clauses_wl S)!C);
+        ASSERT (f = None \<longleftrightarrow> (\<forall>L\<in>#mset (unwatched_l ((get_clauses_wl S)!C)). - L \<in> lits_of_l (get_trail_wl S)));
+        case f of
+          None \<Rightarrow>
+            if val_L' = Some False
+            then do {RETURN (w+1, mark_conflict_wl ((get_clauses_wl S)!C) S)}
+            else do {RETURN (w+1, propgate_lit_wl L' C S)}
+        | Some f \<Rightarrow> do {
+            update_clause_wl L C w i f S
+          }
+      }
+   }\<close>
+lemma \<open>f \<le> \<Down> Id f\<close>
+oops
+declare Id_refine[refine_vcg del] refine0(5)[refine_vcg del]
+
+lemma (in -) mset_tl_update_swap:
   \<open>i < length xs \<Longrightarrow> j < length (xs ! i) \<Longrightarrow> k < length (xs ! i) \<Longrightarrow>
   mset `# mset (tl (xs [i := swap (xs ! i) j k])) = mset `# mset (tl xs)\<close>
   apply (cases i)
@@ -431,12 +412,18 @@ proof -
     if \<open>M = M'\<close> and \<open>L = L'\<close>
     for M M' :: \<open>(nat literal, nat literal, nat) annotated_lit list\<close> and L L'
     using that by (auto simp: valued_def)
-  have find_unwatched: \<open>find_unwatched M (N ! (W K ! w))
-    \<le> \<Down> Id (find_unwatched M' (N' ! (W' K ! w)))\<close>
+  define find_unwatched_wl :: \<open>(nat,nat) ann_lits \<Rightarrow> _\<close> where
+    \<open>find_unwatched_wl = find_unwatched_l\<close>
+  have find_unwatched: \<open>find_unwatched_wl M (N ! (W K ! w))
+    \<le> \<Down> {(L, L'). L = L' \<and> (L \<noteq> None \<longrightarrow> the L < length (N ! (W K ! w)) \<and> the L \<ge> 2)}
+        (find_unwatched_l M' (N' ! (W' K ! w)))\<close>
+      (is \<open>_ \<le> \<Down> ?find_unwatched _\<close>)
     if \<open>N=N'\<close> and \<open>M = M'\<close> and \<open>W = W'\<close>
     for N N' :: \<open>nat literal list list\<close> and
       M M' :: \<open>(nat literal, nat literal, nat) annotated_lit list\<close> and W W'
-    by (auto simp: that)
+    unfolding find_unwatched_l_def find_unwatched_wl_def
+    by (auto simp: that intro: RES_refine)
+
   have \<open>mset `# mset (take n (tl xs)) +
     mset `# mset (drop (Suc n) xs) =
     mset `# mset (tl xs)\<close> for n :: nat and xs :: \<open>'a list list\<close>
@@ -460,19 +447,48 @@ proof -
       using that
       by (simp add: S clauses_def mset_take_mset_drop_mset' m in_all_lits_of_mm_ain_atms_of_iff)
   qed
+  have N_W_K_w_0: \<open>0 < length (N ! (W K ! w))\<close>
+    sorry
+  have \<open>update_clause_wl K (watched_by S K ! w) w
+     (if get_clauses_wl S ! (watched_by S K ! w) ! 0 = K then 0 else 1) n S
+    \<le> ⇓ {((n', T'), n, T). n' = n \<and> T = T' \<and> literals_are_N\<^sub>0 T'}
+       (update_clause_wl K (watched_by S K ! w) w
+         (if get_clauses_wl S ! (watched_by S K ! w) ! 0 = K then 0 else 1) n' S)\<close>
+    if \<open>(n, n') \<in> Id\<close> and \<open>unit_prop_body_wl_D_inv S w K\<close> \<open>(f, f') \<in> ?find_unwatched N W\<close> and
+    \<open>f = Some n\<close> \<open>f' = Some n'\<close>
+    for n n'
+    unfolding update_clause_wl_def S
+    apply clarify
+    apply refine_vcg
+    using that N\<^sub>0 apply (auto simp: clauses_def  mset_take_mset_drop_mset
+          mset_take_mset_drop_mset' m S unit_prop_body_wl_D_inv_def unit_prop_body_wl_inv_def)
+          apply (subst mset_tl_update_swap)
+          apply assumption
+          using N_W_K_w_0 apply assumption
+          apply auto
+          sorry
+          thm literals_are_in_N\<^sub>0_nth additional_WS_invs_def find_unwatched["to_\<Down>"] 
+          find_theorems list_update tl 
   show ?thesis
-    unfolding unit_propagation_inner_loop_body_wl_D_def unit_propagation_inner_loop_body_wl_def S
-      watched_by.simps
+    unfolding unit_propagation_inner_loop_body_wl_D_def find_unwatched_wl_def[symmetric]
+    unfolding unit_propagation_inner_loop_body_wl_def
+    
     supply [[goals_limit=1]]
-    apply (refine_vcg valued find_unwatched f')
-    subgoal using assms unfolding S by fast
+    apply (refine_rcg valued find_unwatched f')
+    subgoal using assms unfolding S unit_prop_body_wl_D_inv_def by auto
     subgoal by simp
-    subgoal using K .
-    subgoal by simp
-    subgoal by simp
+    subgoal by (auto simp: unit_prop_body_wl_D_inv_def)
     subgoal by simp
     subgoal by simp
     subgoal by simp
+    subgoal by simp
+    subgoal by simp
+    subgoal by simp
+    subgoal by (auto simp: mark_conflict_wl_def S unit_prop_body_wl_D_inv_def clauses_def)
+    subgoal by (auto simp: propgate_lit_wl_def S unit_prop_body_wl_D_inv_def clauses_def)
+    subgoal using N\<^sub>0 apply (auto simp: cdcl\<^sub>W_restart_mset_state mset_take_mset_drop_mset'
+          clauses_def image_image m all_lits_of_mm_union is_N\<^sub>1_def S)
+    oops
     subgoal by simp
     subgoal by simp
     subgoal by simp
